utp/utp_hoare.thy
@@ -17,7 +17,7 @@ lemma hoare_r_conj [hoare]: "\<lbrakk> \<lbrace>p\<rbrace>Q\<lbrace>r\<rbrace>\<
 lemma hoare_r_conseq [hoare]: "\<lbrakk> `p\<^sub>1 \<Rightarrow> p\<^sub>2`; \<lbrace>p\<^sub>2\<rbrace>S\<lbrace>q\<^sub>2\<rbrace>\<^sub>u; `q\<^sub>2 \<Rightarrow> q\<^sub>1` \<rbrakk> \<Longrightarrow> \<lbrace>p\<^sub>1\<rbrace>S\<lbrace>q\<^sub>1\<rbrace>\<^sub>u"
   by rel_tac
 
-lemma assigns_hoare_r [hoare]: "\<sigma> \<dagger> q = p \<Longrightarrow> \<lbrace>p\<rbrace>\<langle>\<sigma>\<rangle>\<^sub>a\<lbrace>q\<rbrace>\<^sub>u"
+lemma assigns_hoare_r [hoare]: "`p \<Rightarrow> \<sigma> \<dagger> q` \<Longrightarrow> \<lbrace>p\<rbrace>\<langle>\<sigma>\<rangle>\<^sub>a\<lbrace>q\<rbrace>\<^sub>u"
   by rel_tac
 
 lemma skip_hoare_r [hoare]: "\<lbrace>p\<rbrace>II\<lbrace>p\<rbrace>\<^sub>u"
